Regex/Basic.lean
@@ -4,8 +4,9 @@ import Mathlib.Data.Nat.Notation
 import Mathlib.Computability.Language
 import Mathlib.Computability.RegularExpressions
 import Mathlib.Tactic
-import Regex.Algorithm.PosTermination
+import Regex.Algorithm.Termination
 import Regex.List
+import Regex.Util
 
 namespace Regex
 
@@ -34,9 +35,136 @@ def initMatchPartial (r : Regex α) (w : List α) (s : Pos w) (cap : Captures w)
 def Terminates (r : Regex α) (w : List α) (s : Pos w) (cap : Captures w) :=
   (r.initMatchPartial w s cap).Terminates
 
+/-! Some tactics for proving termination -/
+
+section Tactic
+
+open Lean Parser Tactic
+
+syntax stepArgs :=
+  (&" only")?
+  (" [" withoutPosition((simpStar <|> simpErase <|> simpLemma),*,?) "]")?
+  (location)?
+
+/-- Steps a match stack -/
+syntax "step" stepArgs : tactic
+syntax "step" stepArgs : conv
+
+macro_rules
+| `(tactic| step only $[[$args,*]]? $[$pos:location]?) => `(tactic|
+  (first
+  | rw [MatchStack.step_terminates_iff, MatchStack.Terminates'.eq_def] $[$pos]?
+  | rw [MatchStack.run_eq_step_run] $[$pos]?);
+  simp only [MatchStack.step, Action.process] $[$pos]?;
+  try simp only $[[$args,*]]? $[$pos]?)
+| `(tactic| step $[[$args,*]]? $[$pos:location]?) => `(tactic|
+  (first
+  | rw [MatchStack.step_terminates_iff, MatchStack.Terminates'.eq_def] $[$pos]?
+  | rw [MatchStack.run_eq_step_run] $[$pos]?);
+  simp only [MatchStack.step, Action.process] $[$pos]?;
+  try simp $[[$args,*]]? $[$pos]?)
+| `(tactic| step only $[[$args,*]]?) => `(tactic| step only $[[$args,*]]? at ⊢)
+| `(tactic| step $[[$args,*]]?) => `(tactic| step $[[$args,*]]? at ⊢)
+
+macro_rules
+| `(conv| step only $[[$args,*]]?) => `(conv|
+  (first
+  | rw [MatchStack.step_terminates_iff, MatchStack.Terminates'.eq_def]
+  | rw [MatchStack.run_eq_step_run]) <;>
+  simp only [MatchStack.step, Action.process] <;>
+  try simp only $[[$args,*]]?)
+| `(conv| step $[[$args,*]]?) => `(conv|
+  (first
+  | rw [MatchStack.step_terminates_iff, MatchStack.Terminates'.eq_def]
+  | rw [MatchStack.run_eq_step_run]) <;>
+  simp only [MatchStack.step, Action.process] <;>
+  try simp $[[$args,*]]?)
+
+/-- Runs the top action of a match stack -/
+syntax "run_top" (&" only")?
+  (" [" withoutPosition((simpStar <|> simpErase <|> simpLemma),*,?) "]")?
+  (" at " term (" with " ident ident)?)? : tactic
+syntax "run_top" (&" only")?
+  (" [" withoutPosition((simpStar <|> simpErase <|> simpLemma),*,?) "]")?
+  " using " term : tactic
+
+macro_rules
+| `(tactic| run_top only $[[$args,*]]? at $pos:term with $a:ident $b:ident) => `(tactic|
+    rw [MatchStack.top_run_terminates_iff (by simp only; rfl)] at $pos:term;
+    have tmp := $pos;
+    clear $pos:term;
+    have ⟨$a, $b⟩ := tmp;
+    clear tmp;
+    simp only $[[$args,*]]? at $a $b;
+  )
+| `(tactic| run_top only $[[$args,*]]? $[at $pos:term]?) => `(tactic|
+    (first
+    | rw [MatchStack.top_run_terminates_iff (by simp only; rfl)] $[at $pos:term]?
+    | rw [run_eq_top_run (by simp only; rfl)] $[at $pos:term]?);
+    simp only $[[$args,*]]? $[at $pos:term]?
+)
+| `(tactic| run_top only $[[$args,*]]? using $pos:term) => `(tactic|
+    rw [MatchStack.top_run_terminates_iff (by simp only; rfl)];
+    use $pos:term;
+    simp only $[[$args,*]]?
+  )
+| `(tactic| run_top $[[$args,*]]? at $pos:term with $a:ident $b:ident) => `(tactic|
+    rw [MatchStack.top_run_terminates_iff (by simp only; rfl)] at $pos:term;
+    have tmp := $pos;
+    clear $pos:term;
+    have ⟨$a, $b⟩ := tmp;
+    clear tmp;
+    simp $[[$args,*]]? at $a $b;
+  )
+| `(tactic| run_top $[[$args,*]]? $[at $pos:term]?) => `(tactic|
+    (first
+    | rw [MatchStack.top_run_terminates_iff (by simp only; rfl)] $[at $pos:term]?
+    | rw [MatchStack.run_eq_top_run (by simp only; rfl)] $[at $pos:term]?);
+    simp $[[$args,*]]? $[at $pos:term]?
+)
+| `(tactic| run_top $[[$args,*]]? using $pos:term) => `(tactic|
+    rw [MatchStack.top_run_terminates_iff (by simp only; rfl)];
+    use $pos:term;
+    simp $[[$args,*]]?
+  )
+
+syntax "run_top!" (&" only")?
+  (" [" withoutPosition((simpStar <|> simpErase <|> simpLemma),*,?) "]")?
+  (" at " term (" with " ident ident)?)? : tactic
+syntax "run_top!" (&" only")?
+  (" [" withoutPosition((simpStar <|> simpErase <|> simpLemma),*,?) "]")?
+  " using " term  : tactic
+
+macro_rules
+| `(tactic| run_top! only $[[$args,*]]? at $pos:term with $a:ident $b:ident) => `(tactic|
+    rw! [← List.singleton_append] at $pos:term;
+    run_top only $[[$args,*]]? at $pos with $a $b
+  )
+| `(tactic| run_top! only $[[$args,*]]? $[at $pos:term]?) => `(tactic|
+    rw! [← List.singleton_append] $[at $pos:term]?;
+    run_top only $[[$args,*]]? $[at $pos]?
+  )
+| `(tactic| run_top! only $[[$args,*]]? using $pos:term) => `(tactic|
+    rw! [← List.singleton_append];
+    run_top only $[[$args,*]]? using $pos
+  )
+| `(tactic| run_top! $[[$args,*]]? at $pos:term with $a:ident $b:ident) => `(tactic|
+    rw! [← List.singleton_append] at $pos:term;
+    run_top $[[$args,*]]? at $pos with $a $b
+  )
+| `(tactic| run_top! $[[$args,*]]? $[at $pos:term]?) => `(tactic|
+    rw! [← List.singleton_append] $[at $pos:term]?;
+    run_top $[[$args,*]]? $[at $pos]?
+  )
+| `(tactic| run_top! $[[$args,*]]? using $pos:term) => `(tactic|
+    rw! [← List.singleton_append];
+    run_top $[[$args,*]]? using $pos
+  )
+
+end Tactic
+
 --omit deq in
---open MatchStack in
---theorem initMatchPartial_lawful : (r.initMatchPartial w s cap).Lawful := by
+----theorem initMatchPartial_lawful : (r.initMatchPartial w s cap).Lawful := by
 --  apply Lawful.mk
 --  all_goals simp only [initMatchPartial]
 --  · simp [posLawful_sorted]
@@ -49,297 +177,517 @@ def Terminates (r : Regex α) (w : List α) (s : Pos w) (cap : Captures w) :=
 --    all_goals simp [Action.posLawful_le_arg, Action.posLawful_lt_arg_filterEmpty]
 --  · simp [posLawful_consecutive]
 
-open MatchStack in
+section MatchPartial
+open MatchStack
+
 def matchPartial (r : Regex α) (w : List α) (s : Pos w) (cap : Captures w)
   (term : r.Terminates w s cap)
-    : PartialMatches w := T.run ⟨
-      (r.initMatchPartial w s cap), term
-    ⟩
+    : PartialMatches w := (r.initMatchPartial w s cap).run term
 
-open MatchStack in
+theorem matchPartial_terminates_iff {r : Regex α} {w : List α} {s : Pos w} {cap : Captures w}
+    : r.Terminates w s cap ↔ (mk [.regex r s cap] []).Terminates := iff_of_eq rfl
+
+theorem matchPartial_eq_run {r : Regex α} {w : List α} {s : Pos w} {cap : Captures w}
+  {term : r.Terminates w s cap}
+    : r.matchPartial w s cap term = (mk [.regex r s cap] []).run term := rfl
+
+/-- `bot` always terminates -/
 theorem matchPartial_bot_terminates (s : Pos w) (cap : Captures w)
     : [/⊥/].Terminates w s cap := by
-  apply terminates_of_stepN (n := 2) (mat := [])
-  simp [stepN, step, initMatchPartial, Action.process, Except.ok_eq_pure]
+  rw [Terminates, initMatchPartial]; step; step
 
-open MatchStack in
+/-- `empty` always terminates -/
 theorem matchPartial_empty_terminates (s : Pos w) (cap : Captures w)
     : [//].Terminates w s cap := by
-  apply terminates_of_stepN (n := 2) (mat := [(s, cap)])
-  simp [stepN, step, initMatchPartial, Action.process, Except.ok_eq_pure]
+  rw [Terminates, initMatchPartial]; step; step
 
-open MatchStack in
+/-- `unit` always terminates -/
 theorem matchPartial_unit_terminates (c : α) (s : Pos w) (cap : Captures w)
     : [/c/].Terminates w s cap := by
-  apply terminates_of_stepN (n := 2)
-    (mat := if h : w[s.val]? = some c then [(s.succOfIndex h, cap)] else [])
-  simp [stepN, step, initMatchPartial, Action.process, Except.ok_eq_pure]
+  rw [Terminates, initMatchPartial]; step; step
 
-open MatchStack in
+theorem Action.concat_terminates {r : Regex α} {s : Pos w}
+    {old new arg : PartialMatches w}
+    : (MatchStack.mk [concat r s old new] arg).Terminates ↔
+      ∀ mat ∈ old, r.Terminates w mat.1 mat.2 := by
+  constructor
+  · intro term mat mem
+    induction old generalizing s new arg with | nil => contradiction | cons ent mat' ind =>
+      step at term
+      run_top! at term with term' term
+      rw [List.mem_cons] at mem
+      rcases mem with mem | mem
+      · exact mem ▸ term'
+      · exact ind term mem
+  · intro term
+    induction old generalizing s new arg with | nil => step; step | cons ent mat' ind =>
+      step
+      run_top!
+      use term ent List.mem_cons_self
+      exact ind fun m mem ↦ term _ (List.mem_cons_of_mem _ mem)
+
+theorem Action.concatWait_terminates {q r : Regex α} {s : Pos w} {arg : PartialMatches w}
+    : (MatchStack.mk [concatWait q r s] arg).Terminates ↔
+      ∀ mat ∈ arg, r.Terminates w mat.1 mat.2 := by
+  constructor
+  · intro term mat mem
+    step at term
+    cases arg with | nil => contradiction | cons ent mat' =>
+      simp only [reduceCtorEq, ↓reduceDIte, List.map_cons] at term
+      rw [concat_terminates] at term
+      exact term mat mem
+  · intro term
+    step
+    cases arg with | nil => step | cons ent mat' =>
+      simp only [reduceCtorEq, ↓reduceDIte, List.map_cons]
+      rwa [concat_terminates]
+
+/-- `concat q r` terminates iff `q` terminates and `r` terminates for every
+end position and match provided by `q` -/
 theorem matchPartial_concat_terminates {q r : Regex α} {s : Pos w} {cap : Captures w}
-    : [/⟨q⟩ ⟨r⟩/].Terminates w s cap ↔ ∃ term : q.Terminates w s cap,
+    : [/⟨q⟩ ⟨r⟩/].Terminates w s cap ↔ (term : q.Terminates w s cap) ∧
       ∀ mat ∈ q.matchPartial w s cap term, r.Terminates w mat.1 mat.2 := by
   constructor
   · intro term
     rw [Terminates, initMatchPartial] at term
-    have hst' : (mk [Action.regex [/⟨q⟩ ⟨r⟩/] s cap] []).step = ?_ := by
-      simp only [step, Action.process, List.append_nil]; rfl
-    have term' := step_terminates term hst'
-    have qterm := top_terminates term' (by simp only; rw [← List.singleton_append])
-    simp only at qterm
-    use qterm
+    step at term
+    run_top! at term with term' term
+    use term'
     intro mat qmat
-    have run := top_run_terminates term'
-    --have term'' := step_terminates' term'; simp [step] at term''
-    --have term'' := step_terminates' term''; simp [step] at term''
+    rw [matchPartial] at qmat
+    rw [Action.concatWait_terminates] at term
+    exact term mat qmat
+  · rintro ⟨qterm, term⟩
+    rw [Terminates, initMatchPartial] at ⊢
+    step
+    run_top! using qterm
+    rw [Action.concatWait_terminates]
+    exact fun mat run ↦ term mat run
 
-open MatchStack in
+theorem Action.or_terminates {s : Pos w} {fst arg : PartialMatches w}
+    : (MatchStack.mk [or s fst] arg).Terminates := by step; step
+
+theorem Action.orWait_terminates {r : Regex α} {s : Pos w} {cap : Captures w}
+    {arg : PartialMatches w}
+    : (MatchStack.mk [orWait r s cap] arg).Terminates ↔ r.Terminates w s cap := by
+  constructor
+  · intro term
+    step at term
+    run_top! at term with term' term
+    exact term'
+  · intro term
+    step
+    run_top! using term
+    exact or_terminates
+
+/-- `or q r` terminates iff `q` terminates and `r` terminates -/
+theorem matchPartial_or_terminates {q r : Regex α} {s : Pos w} {cap : Captures w}
+    : [/⟨q⟩ | ⟨r⟩/].Terminates w s cap ↔
+      q.Terminates w s cap ∧ r.Terminates w s cap := by
+  constructor
+  · intro term
+    rw [Terminates, initMatchPartial] at term
+    step at term
+    run_top! at term with term' term
+    exact ⟨term', Action.orWait_terminates.mp term⟩
+  · rintro ⟨qterm, rterm⟩
+    rw [Terminates, initMatchPartial]
+    step
+    run_top! using qterm
+    exact Action.orWait_terminates.mpr rterm
+
+theorem Action.filterEmpty_terminates {emp : Bool} {s : Pos w} {arg : PartialMatches w}
+    : (MatchStack.mk [filterEmpty emp s] arg).Terminates := by step; step
+
+/-- `filterEmpty emp r` terminates iff `r` terminates -/
+theorem matchPartial_filterEmpty_terminates {emp : Bool} {r : Regex α}
+    {s : Pos w} {cap : Captures w}
+    : [/⟨r⟩ ‹emp›ε/].Terminates w s cap ↔ r.Terminates w s cap := by
+  constructor <;> intro term
+  · rw [Terminates, initMatchPartial] at term
+    step at term
+    run_top! at term
+    exact term.1
+  · rw [Terminates, initMatchPartial]
+    step
+    run_top!
+    exact ⟨term, Action.filterEmpty_terminates⟩
+
+theorem Action.capture_terminates {n : ℕ} {s : Pos w} {arg : PartialMatches w}
+    : (MatchStack.mk [capture n s] arg).Terminates := by step; step
+
+/-- `capture emp r` terminates iff `r` terminates -/
+theorem matchPartial_capture_terminates {n : ℕ} {r : Regex α}
+    {s : Pos w} {cap : Captures w}
+    : [/(‹n› ⟨r⟩)/].Terminates w s cap ↔ r.Terminates w s cap := by
+  constructor <;> intro term
+  · rw [Terminates, initMatchPartial] at term
+    step at term
+    run_top! at term
+    exact term.1
+  · rw [Terminates, initMatchPartial]
+    step
+    run_top!
+    exact ⟨term, Action.capture_terminates⟩
+
 theorem matchPartial_bot (s : Pos w) (cap : Captures w)
     : matchPartial [/⊥/] w s cap (matchPartial_bot_terminates s cap) = [] := by
-  simp only [matchPartial, initMatchPartial]
-  rw [T.run, T.step]
-  simp only [step, Action.process, List.extract_eq_drop_take, ↓dreduceDIte,
-    List.filter_nil, List.map_nil, List.nil_append]
-  rw [T.run, T.step]
-  simp [step]
+  simp only [matchPartial_eq_run]; step; step
 
-open MatchStack in
 theorem matchPartial_empty (s : Pos w) (cap : Captures w)
     : matchPartial [//] w s cap (matchPartial_empty_terminates s cap)
     = [(s, cap)] := by
-  simp only [matchPartial, initMatchPartial]
-  rw [T.run, T.step]
-  simp only [step, Action.process, List.extract_eq_drop_take, ↓dreduceDIte,
-    List.filter_nil, List.map_nil, List.nil_append]
-  rw [T.run, T.step]
-  simp [step]
+  simp only [matchPartial_eq_run]; step; step
 
-open MatchStack in
 theorem matchPartial_unit (c : α) (s : Pos w) (cap : Captures w)
     : matchPartial [/c/] w s cap (matchPartial_unit_terminates c s cap)
       = if h : w[s.val]? = some c then [(s.succOfIndex h, cap)] else [] := by
-  simp only [matchPartial, initMatchPartial]
-  rw [T.run, T.step]
-  simp only [step, Action.process, List.extract_eq_drop_take, ↓dreduceDIte,
-    List.filter_nil, List.map_nil, List.nil_append]
-  rw [T.run, T.step]
-  simp [step]
+  simp only [matchPartial_eq_run]; step; step
 
-open MatchStack in
+theorem Action.concat_run {r : Regex α} {s : Pos w} {old new arg : PartialMatches w}
+    (term : ∀ mat ∈ old, r.Terminates w mat.1 mat.2)
+    : (mk [.concat r s old new] arg).run (concat_terminates.mpr term)
+      = new ++ arg ++
+      (old.pmap (fun ent rt ↦ r.matchPartial w ent.1 ent.2 rt) term).flatten := by
+  induction old generalizing new arg with | nil => step; step | cons ent mat ind =>
+    simp only [List.mem_cons, forall_eq_or_imp, List.pmap_cons,
+      List.flatten_cons] at term ⊢
+    step
+    run_top!
+    rw [ind term.2]
+    simp only [List.append_assoc, List.append_cancel_left_eq,
+      List.append_cancel_right_eq]
+    rfl
+
+theorem Action.concatWait_run {q r : Regex α} {s : Pos w} {arg : PartialMatches w}
+    (term : ∀ mat ∈ arg, r.Terminates w mat.1 mat.2)
+    : (mk [.concatWait q r s] arg).run (concatWait_terminates.mpr term)
+      = (arg.pmap (fun ent rt ↦ r.matchPartial w ent.1 ent.2 rt) term).flatten := by
+  step
+  cases arg with | nil => step | cons ent mat =>
+    simp only [reduceCtorEq, ↓reduceDIte, List.map_cons, List.pmap_cons,
+      List.flatten_cons]
+    simp [concat_run term]
+
 theorem matchPartial_concat (q r : Regex α) (s : Pos w) (cap : Captures w)
     (term : [/⟨q⟩ ⟨r⟩/].Terminates w s cap)
     : matchPartial [/⟨q⟩ ⟨r⟩/] w s cap term
-      = q.matchPartial w s cap >>= fun (s', cap') ↦ r.matchPartial w s' cap' := by
-  sorry
+      = ((q.matchPartial w s cap (matchPartial_concat_terminates.mp term).1).pmap
+          (fun ent rt ↦ r.matchPartial w ent.1 ent.2 rt)
+            (matchPartial_concat_terminates.mp term).2).flatten := by
+  rw [matchPartial]
+  simp only [initMatchPartial]
+  step
+  run_top!
+  rw! [← matchPartial_eq_run]
+  rw [Action.concatWait_run (matchPartial_concat_terminates.mp term).2]
 
---theorem MatchStack.T.step_run {st st' : MatchStack.T w}
---    (hst : st.step = Except.ok st')
---    : st.run = st'.run := by
+theorem Action.or_run {s : Pos w} {fst arg : PartialMatches w}
+    : (mk [.or s fst] arg).run or_terminates = fst ++ arg := by step; step
 
-def match' (r : Regex α) (w : List α) (term : r.isTerminating w 0 0) :
-  PartialMatches w := r.matchPartial w 0 0 term
+theorem Action.orWait_run {r : Regex α} {s : Pos w} {cap : Captures w}
+    {arg : PartialMatches w} (term : r.Terminates w s cap)
+    : (mk [.orWait r s cap] arg).run (orWait_terminates.mpr term)
+      = arg ++ r.matchPartial w s cap term := by step; run_top!; step; step; rfl
 
-#eval runMatch [/(1 ← 0 | 1)/] [0, 1, 2, 3] 100
+theorem matchPartial_or (q r : Regex α) (s : Pos w) (cap : Captures w)
+    (term : [/⟨q⟩ | ⟨r⟩/].Terminates w s cap)
+    : matchPartial [/⟨q⟩ | ⟨r⟩/] w s cap term
+      = q.matchPartial w s cap (matchPartial_or_terminates.mp term).1 ++
+        r.matchPartial w s cap (matchPartial_or_terminates.mp term).2 := by
+  rw [matchPartial]
+  simp only [initMatchPartial]
+  step
+  run_top!
+  rw [Action.orWait_run (matchPartial_or_terminates.mp term).2]
+  rfl
 
-mutual
---def matchPartialStar (t : StarType) (r : Regex α) (w : List α) (s : Pos w) (cap : Captures w)
+theorem Action.filterEmpty_run {emp : Bool} {s : Pos w} {arg : PartialMatches w}
+    : (mk [.filterEmpty emp s] arg).run filterEmpty_terminates
+      = arg.filter fun ent => (s = ent.1) = emp := by step; step
+
+theorem matchPartial_filterEmpty (emp : Bool) (r : Regex α) (s : Pos w) (cap : Captures w)
+    (term : [/⟨r⟩ ‹emp›ε/].Terminates w s cap)
+    : matchPartial [/⟨r⟩ ‹emp›ε/] w s cap term =
+      (r.matchPartial w s cap (matchPartial_filterEmpty_terminates.mp term)).filter
+        fun ent ↦ (s = ent.1) = emp := by
+  rw [matchPartial]
+  simp only [initMatchPartial]
+  step
+  run_top!
+  simp only [Action.filterEmpty_run, eq_iff_iff, Bool.decide_iff_dist, Bool.decide_eq_true]
+  rfl
+
+theorem matchPartial_star_greedy_terminates' {r : Regex α} {s : Pos w}
+    {cap : Captures w}
+    : [/⟨r⟩*/].Terminates w s cap ↔
+      [/(⟨r⟩ •ε | (⟨r⟩ -ε) ⟨r⟩*) | ε/].Terminates w s cap := by
+  simp only [Terminates, initMatchPartial]; conv_lhs => step
+
+theorem matchPartial_star_lazy_terminates' {r : Regex α} {s : Pos w}
+    {cap : Captures w}
+    : [/⟨r⟩*?/].Terminates w s cap ↔
+      [/ε | (⟨r⟩ •ε | (⟨r⟩ -ε) ⟨r⟩*?)/].Terminates w s cap := by
+  simp only [Terminates, initMatchPartial]; conv_lhs => step
+
+/-- `star t r` terminates iff `r` terminates and `r` terminates for every
+advancing end position and match provided by `r` -/
+theorem matchPartial_star_terminates {t : StarType} {r : Regex α} {s : Pos w}
+    {cap : Captures w}
+    : [/⟨r⟩*‹t›/].Terminates w s cap ↔ (term : r.Terminates w s cap) ∧
+      ∀ mat ∈ r.matchPartial w s cap term,
+        s ≠ mat.1 → [/⟨r⟩*‹t›/].Terminates w mat.1 mat.2 := by
+  rw [Terminates, initMatchPartial]
+  step only [List.append_nil]
+  cases t with
+  | greedy =>
+    simp only
+    rw [← matchPartial_terminates_iff, matchPartial_or_terminates,
+      matchPartial_or_terminates] at ⊢
+    rw! [matchPartial_filterEmpty_terminates, matchPartial_concat_terminates,
+      matchPartial_filterEmpty_terminates]
+    simp [dand_iff_and_forall, matchPartial_empty_terminates, matchPartial_filterEmpty]
+  | lazy =>
+    simp only
+    rw [← matchPartial_terminates_iff, matchPartial_or_terminates,
+      matchPartial_or_terminates] at ⊢
+    rw! [matchPartial_filterEmpty_terminates, matchPartial_concat_terminates,
+      matchPartial_filterEmpty_terminates]
+    simp [dand_iff_and_forall, matchPartial_empty_terminates, matchPartial_filterEmpty]
+
+theorem matchPartial_star (t : StarType) (r : Regex α) (s : Pos w) (cap : Captures w)
+    (term : [/⟨r⟩*‹t›/].Terminates w s cap)
+    : matchPartial [/⟨r⟩*‹t›/] w s cap term = match t with
+      | .greedy => [/(⟨r⟩ •ε | (⟨r⟩ -ε) ⟨r⟩*) | ε/].matchPartial w s cap
+        (matchPartial_star_greedy_terminates'.mp term)
+      | .lazy => [/ε | (⟨r⟩ •ε | (⟨r⟩ -ε) ⟨r⟩*?)/].matchPartial w s cap
+        (matchPartial_star_lazy_terminates'.mp term)
+      := by
+  simp only [matchPartial_eq_run]
+  split <;> conv_lhs => step
+
+theorem Action.capture_run {n : ℕ} {s : Pos w} {arg : PartialMatches w}
+    : (mk [.capture n s] arg).run capture_terminates
+      = arg.map fun ent ↦ (ent.1, ent.2.update n [(s, ent.1)]) := by step; step
+
+theorem matchPartial_capture (n : ℕ) (r : Regex α) (s : Pos w) (cap : Captures w)
+    (term : [/(‹n› ⟨r⟩)/].Terminates w s cap)
+    : matchPartial [/(‹n› ⟨r⟩)/] w s cap term =
+      (r.matchPartial w s cap (matchPartial_capture_terminates.mp term)).map
+        fun ent ↦ (ent.1, ent.2.update n [(s, ent.1)]) := by
+  rw [matchPartial]
+  simp only [initMatchPartial]
+  step
+  run_top!
+  simp only [Action.capture_run]
+  rfl
+
+end MatchPartial
+
+--def match' (r : Regex α) (w : List α) (term : r.isTerminating w 0 0) :
+--  PartialMatches w := r.matchPartial w 0 0 term
+--
+--#eval runMatch [/(1 ← 0 | 1)/] [0, 1, 2, 3] 100
+
+--mutual
+----def matchPartialStar (t : StarType) (r : Regex α) (w : List α) (s : Pos w) (cap : Captures w)
+----    : List (IccFrom s × Captures w) :=
+----  matchPartial r w s cap >>=
+----  /- Matching an empty string means you can't continue -/
+----    fun (s', cap') ↦ if s.val = s'.val then pure (s', cap') else
+----      (fun (s'', cap'') ↦ (s'.widenLeft s'', cap'')) <$>
+----      matchPartial (star t r) w s'.expandZero cap'
+----termination_by (star t r, s.distToEnd, 0)
+----decreasing_by
+----  · simp only [Prod.lex_def, star.sizeOf_spec, Nat.lt_add_left_iff_pos, Nat.lt_irrefl,
+----      Nat.not_lt_zero, and_false, or_self, or_false]
+----    exact Nat.lt_add_right (sizeOf t) Nat.zero_lt_one
+----  · rename_i hs
+----    simp only [Prod.lex_def, star.sizeOf_spec, Nat.lt_irrefl, Nat.not_lt_zero, and_false,
+----      or_false, true_and, false_or]
+----    apply Icc.distToEnd_lt
+----    rcases lt_or_eq_of_le s'.is_ge with slt | seq
+----    · exact slt
+----    · contradiction
+--
+--/-- Partial match: takes a regex, a string, a start position, and a list of
+--current captures, and returns a list of possible matches to check in order.
+--Each match is an end position combined with a capture list. -/
+--partial def matchPartial (r : Regex α) (w : List α) (s : Pos w) (cap : Captures w)
 --    : List (IccFrom s × Captures w) :=
---  matchPartial r w s cap >>=
---  /- Matching an empty string means you can't continue -/
---    fun (s', cap') ↦ if s.val = s'.val then pure (s', cap') else
---      (fun (s'', cap'') ↦ (s'.widenLeft s'', cap'')) <$>
---      matchPartial (star t r) w s'.expandZero cap'
---termination_by (star t r, s.distToEnd, 0)
---decreasing_by
---  · simp only [Prod.lex_def, star.sizeOf_spec, Nat.lt_add_left_iff_pos, Nat.lt_irrefl,
---      Nat.not_lt_zero, and_false, or_self, or_false]
---    exact Nat.lt_add_right (sizeOf t) Nat.zero_lt_one
---  · rename_i hs
---    simp only [Prod.lex_def, star.sizeOf_spec, Nat.lt_irrefl, Nat.not_lt_zero, and_false,
---      or_false, true_and, false_or]
---    apply Icc.distToEnd_lt
---    rcases lt_or_eq_of_le s'.is_ge with slt | seq
---    · exact slt
---    · contradiction
-
-/-- Partial match: takes a regex, a string, a start position, and a list of
-current captures, and returns a list of possible matches to check in order.
-Each match is an end position combined with a capture list. -/
-partial def matchPartial (r : Regex α) (w : List α) (s : Pos w) (cap : Captures w)
-    : List (IccFrom s × Captures w) :=
-  match r with
-  | bot => failure
-  | empty => pure (s.iccFrom, cap)
-  | unit c => if hs : w[s.val]? = c then pure (Icc.succOfIndex hs, cap) else failure
-  | concat q r => do
-      let (s', cap') ← q.matchPartial w s cap
-      let (s'', cap'') ← r.matchPartial w s'.expandZero cap'
-      pure (s'.widenLeft s'', cap'')
-  | or q r => q.matchPartial w s cap ++ r.matchPartial w s cap
-  | filterEmpty emp r => do
-      let (s', cap') ← r.matchPartial w s cap
-      if (s'.val = s.val) = emp then pure (s', cap') else failure
-  --| star t r => match t with
-  --  | .greedy => matchPartialStar .greedy r w s cap ++ pure (s.iccFrom, cap)
-  --  | .lazy => pure (s.iccFrom, cap) ++ matchPartialStar .lazy r w s cap
-  | star t r => match t with
-    | .greedy => matchPartial [/(¥ᵣ(r) •ε | (¥ᵣ(r) -ε) ¥ᵣ(r)*) | ε/] w s cap
-    | .lazy => matchPartial [/ε | (¥ᵣ(r) •ε | (¥ᵣ(r) -ε) ¥ᵣ(r)*?)/] w s cap
-  | capture n r => do
-      let (s', cap') ← r.matchPartial w s cap
-      pure (s', cap'.update n (pure ⟨s, s'⟩))
-  | backref d n => do
-      let ⟨cs, ct⟩ ← if let some w' := (cap n).getLast? then pure w'
-        else return (← matchPartial d w s cap)
-      if h : w.extract s.val (s.val + (ct.val - cs.val)) = w.extract cs.val ct.val then
-        pure (Icc.addOfIndex h (length_extract_pos_posFrom cs ct), cap) else failure
---termination_by (s.distToEnd, r.numRawStars, r)
---decreasing_by
---  all_goals have sizelt (a b : ℕ) : a < 1 + a + b := by linarith
---  all_goals have zz (n : ℕ) : 0 < n ∨ n = 0 := by omega
---  any_goals simp [Prod.lex_def, numRawStars, sizelt, ← le_iff_lt_or_eq, zz]
-end
-
-theorem matchPartial_bot (w : List α) (s : Pos w) (cap : Captures w)
-    : matchPartial [/⊥/] w s cap = [] := by
-  simp [matchPartial, failure]
-
-theorem matchPartial_empty (w : List α) (s : Pos w) (cap : Captures w)
-    : matchPartial [//] w s cap = [(s.iccFrom, cap)] := by
-  simp [matchPartial]
-
---theorem matchPartial_star_nil (t : StarType) (r : Regex α) (s : Pos []) (cap : Captures [])
---    : Prod.fst <$> (star t r).matchPartial [] s cap =
---      if matchPartial r [] s cap = [] then [s.posFrom] else [s.posFrom, s.posFrom] := by
---  rcases t
---  · simp only [matchPartial, List.pure_def, List.cons_append, List.nil_append,
---      List.map_eq_map, List.map_cons]
---    simp only [matchPartialStar, Prod.mk.eta, List.pure_def, List.map_eq_map,
---      List.bind_eq_flatMap]
---    split_ifs with h
---    · simp [h]
---    ·
-
-/-- A finishing partial match -/
-def matchFinish (r : Regex α) (w : List α) (s : Pos w) (cap : Captures w)
-    : Option (Captures w) :=
-  Prod.snd <$> (matchPartial r w s cap).find? fun (s, _) ↦ s = s.end'
-
-/-- Matches a regex against an entire string.
-Returns a list of captures if it succeeds.
-Called `match'` because `match` is a keyword. -/
-def match' (r : Regex α) (w : List α) : Option (Captures w) := matchFinish r w 0 0
-  --Prod.snd <$> (matchPartial r w 0 0).find? fun (s, _) ↦ s = Pos.end'
-
-theorem match'_bot (w : List α) : match' [/⊥/] w = none := by
-  simp [match', matchFinish, matchPartial_bot]
-
-theorem match'_empty (w : List α) : match' [//] w = if w = [] then some 0 else none := by
-  simp only [match', matchFinish, matchPartial_empty, List.find?_singleton,
-    decide_eq_true_eq, Option.map_eq_map, Option.map_if]
-  congr
-  rw [Icc.zero_end']
-  rfl
-
-theorem match'_unit (c : α) (w : List α)
-    : match' [/c/] w = if w = [c] then some 0 else none := by
-  simp only [match', matchFinish, matchPartial, List.pure_def, Option.map_eq_map]
-  split_ifs with w0c wc wc
-  · simp only [List.find?_singleton, decide_eq_true_eq, Option.map_if,
-      ite_eq_left_iff, reduceCtorEq, imp_false, Decidable.not_not]
-    rw [← Subtype.val_inj]
-    simp [Icc.succOfIndex, wc]
-  · simp only [List.find?_singleton, decide_eq_true_eq, Option.map_if, ite_eq_right_iff,
-      reduceCtorEq, imp_false]
-    contrapose! wc
-    apply_fun Subtype.val at wc
-    simp only [Icc.zero_val, Icc.succOfIndex_val, zero_add, Icc.end'_val] at wc
-    rw [Icc.zero_val] at w0c
-    rw [eq_comm, List.length_eq_one_iff] at wc
-    rcases wc with ⟨a, wa⟩
-    have wa' := congrArg (·[0]?) wa
-    simp only [w0c, List.length_cons, List.length_nil, zero_add, zero_lt_one,
-      getElem?_pos, List.getElem_cons_zero, Option.some.injEq] at wa'
-    exact wa' ▸ wa
-  · simp [wc] at w0c
-  · simp [failure]
-
-theorem match'_concat (q r : Regex α) (w : List α)
-    : match' [/¥ᵣ(q)¥ᵣ(r)/] w = (matchPartial q w 0 0).findSome?
-        (fun (s, cap) ↦ matchFinish r w s cap) := by
-  simp only [match', matchFinish, matchPartial, List.pure_def, List.bind_eq_flatMap,
-    List.find?_flatMap, List.find?_singleton, decide_eq_true_eq, Option.map_eq_map,
-    List.map_findSome?]
-  congr
-  rw [Function.comp_def]
-  ext x cs
-  rw [Option.map_eq_some_iff, Option.map_eq_some_iff]
-  simp only [Prod.exists, exists_eq_right]
-  simp only [List.findSome?_eq_some_iff, Option.ite_none_right_eq_some, Option.some.injEq,
-    Prod.mk.injEq, ite_eq_right_iff, reduceCtorEq, imp_false, Prod.forall,
-    exists_and_right, Prod.exists, ↓existsAndEq, and_true]
-  rw [exists_comm]
-  apply exists_congr; intro s
-  simp only [List.find?_eq_some_iff_append, decide_eq_true_eq, Bool.not_eq_eq_eq_not,
-    Bool.not_true, decide_eq_false_iff_not, Prod.forall, exists_and_right,
-    ← Icc.val_inj]
-  rw [← exists_and_left]
-  apply exists_congr; intro csl
-  rw [and_left_comm]
-  rfl
-
-theorem match'_or (q r : Regex α) (w : List α)
-    : match' (or q r) w = (match' q w <|> match' r w) := by
-  simp only [match', matchFinish, matchPartial, List.find?_append, Option.map_eq_map,
-    Option.orElse_eq_orElse, Option.orElse_eq_or]
-  rw [Option.map_or]
-
-/-- Matching specialized to strings. -/
-def matchStr (r : Regex Char) (w : String) := match' r w.toList
-
-def isMatch (r : Regex α) (w : List α) := ∃ cs, match' r w = some cs
-
-theorem isMatch_bot (w : List α) : ¬isMatch [/⊥/] w := by
-  simp [isMatch, match'_bot]
-
-theorem isMatch_empty (w : List α) : isMatch [//] w ↔ w = [] := by
-  simp [isMatch, match'_empty]
-
-theorem isMatch_unit (c : α) (w : List α) : isMatch [/c/] w ↔ w = [c] := by
-  simp [isMatch, match'_unit]
-
-theorem isMatch_or (q r : Regex α) (w : List α)
-    : isMatch (or q r) w ↔ isMatch q w ∨ isMatch r w := by
-  simp only [isMatch, match'_or, Option.orElse_eq_orElse, Option.orElse_eq_or,
-    Option.or_eq_some_iff]
-  constructor <;> intro excs
-  · rcases excs with ⟨cs, qcs | ⟨q0, rcs⟩⟩
-    · exact Or.inl ⟨cs, qcs⟩
-    · exact Or.inr ⟨cs, rcs⟩
-  · by_cases qcs : ∃ cs, q.match' w = some cs
-    · rcases qcs with ⟨cs, qcs⟩
-      exact ⟨cs, Or.inl qcs⟩
-    · simp only [qcs, false_or] at excs
-      push_neg at qcs
-      rw [← Option.eq_none_iff_forall_ne_some] at qcs
-      rcases excs with ⟨cs, rcs⟩
-      exact ⟨cs, Or.inr ⟨qcs, rcs⟩⟩
-
-def language (r : Regex α) : Language α := {w | isMatch r w}
-
-theorem language_bot (α : Type*) [DecidableEq α] : ([/⊥/] : Regex α).language = 0 := by
-  simp [language, isMatch_bot]
-  rfl
-
-theorem language_empty (α : Type*) [DecidableEq α] : ([//] : Regex α).language = {[]} := by
-  simp [language, isMatch_empty]
-
-theorem language_unit (c : α) : [/c/].language = {[c]} := by
-  simp [language, isMatch_unit]
-
-theorem language_or (q r : Regex α) : (or q r).language = q.language + r.language := by
-  simp [language, isMatch_or, Language.add_def, Set.union_def]
-
-#eval matchStr [/(1 ← ('0' | '1')*) \⊥1/] "011011"
+--  match r with
+--  | bot => failure
+--  | empty => pure (s.iccFrom, cap)
+--  | unit c => if hs : w[s.val]? = c then pure (Icc.succOfIndex hs, cap) else failure
+--  | concat q r => do
+--      let (s', cap') ← q.matchPartial w s cap
+--      let (s'', cap'') ← r.matchPartial w s'.expandZero cap'
+--      pure (s'.widenLeft s'', cap'')
+--  | or q r => q.matchPartial w s cap ++ r.matchPartial w s cap
+--  | filterEmpty emp r => do
+--      let (s', cap') ← r.matchPartial w s cap
+--      if (s'.val = s.val) = emp then pure (s', cap') else failure
+--  --| star t r => match t with
+--  --  | .greedy => matchPartialStar .greedy r w s cap ++ pure (s.iccFrom, cap)
+--  --  | .lazy => pure (s.iccFrom, cap) ++ matchPartialStar .lazy r w s cap
+--  | star t r => match t with
+--    | .greedy => matchPartial [/(¥ᵣ(r) •ε | (¥ᵣ(r) -ε) ¥ᵣ(r)*) | ε/] w s cap
+--    | .lazy => matchPartial [/ε | (¥ᵣ(r) •ε | (¥ᵣ(r) -ε) ¥ᵣ(r)*?)/] w s cap
+--  | capture n r => do
+--      let (s', cap') ← r.matchPartial w s cap
+--      pure (s', cap'.update n (pure ⟨s, s'⟩))
+--  | backref d n => do
+--      let ⟨cs, ct⟩ ← if let some w' := (cap n).getLast? then pure w'
+--        else return (← matchPartial d w s cap)
+--      if h : w.extract s.val (s.val + (ct.val - cs.val)) = w.extract cs.val ct.val then
+--        pure (Icc.addOfIndex h (length_extract_pos_posFrom cs ct), cap) else failure
+----termination_by (s.distToEnd, r.numRawStars, r)
+----decreasing_by
+----  all_goals have sizelt (a b : ℕ) : a < 1 + a + b := by linarith
+----  all_goals have zz (n : ℕ) : 0 < n ∨ n = 0 := by omega
+----  any_goals simp [Prod.lex_def, numRawStars, sizelt, ← le_iff_lt_or_eq, zz]
+--end
+--
+--theorem matchPartial_bot (w : List α) (s : Pos w) (cap : Captures w)
+--    : matchPartial [/⊥/] w s cap = [] := by
+--  simp [matchPartial, failure]
+--
+--theorem matchPartial_empty (w : List α) (s : Pos w) (cap : Captures w)
+--    : matchPartial [//] w s cap = [(s.iccFrom, cap)] := by
+--  simp [matchPartial]
+--
+----theorem matchPartial_star_nil (t : StarType) (r : Regex α) (s : Pos []) (cap : Captures [])
+----    : Prod.fst <$> (star t r).matchPartial [] s cap =
+----      if matchPartial r [] s cap = [] then [s.posFrom] else [s.posFrom, s.posFrom] := by
+----  rcases t
+----  · simp only [matchPartial, List.pure_def, List.cons_append, List.nil_append,
+----      List.map_eq_map, List.map_cons]
+----    simp only [matchPartialStar, Prod.mk.eta, List.pure_def, List.map_eq_map,
+----      List.bind_eq_flatMap]
+----    split_ifs with h
+----    · simp [h]
+----    ·
+--
+--/-- A finishing partial match -/
+--def matchFinish (r : Regex α) (w : List α) (s : Pos w) (cap : Captures w)
+--    : Option (Captures w) :=
+--  Prod.snd <$> (matchPartial r w s cap).find? fun (s, _) ↦ s = s.end'
+--
+--/-- Matches a regex against an entire string.
+--Returns a list of captures if it succeeds.
+--Called `match'` because `match` is a keyword. -/
+--def match' (r : Regex α) (w : List α) : Option (Captures w) := matchFinish r w 0 0
+--  --Prod.snd <$> (matchPartial r w 0 0).find? fun (s, _) ↦ s = Pos.end'
+--
+--theorem match'_bot (w : List α) : match' [/⊥/] w = none := by
+--  simp [match', matchFinish, matchPartial_bot]
+--
+--theorem match'_empty (w : List α) : match' [//] w = if w = [] then some 0 else none := by
+--  simp only [match', matchFinish, matchPartial_empty, List.find?_singleton,
+--    decide_eq_true_eq, Option.map_eq_map, Option.map_if]
+--  congr
+--  rw [Icc.zero_end']
+--  rfl
+--
+--theorem match'_unit (c : α) (w : List α)
+--    : match' [/c/] w = if w = [c] then some 0 else none := by
+--  simp only [match', matchFinish, matchPartial, List.pure_def, Option.map_eq_map]
+--  split_ifs with w0c wc wc
+--  · simp only [List.find?_singleton, decide_eq_true_eq, Option.map_if,
+--      ite_eq_left_iff, reduceCtorEq, imp_false, Decidable.not_not]
+--    rw [← Subtype.val_inj]
+--    simp [Icc.succOfIndex, wc]
+--  · simp only [List.find?_singleton, decide_eq_true_eq, Option.map_if, ite_eq_right_iff,
+--      reduceCtorEq, imp_false]
+--    contrapose! wc
+--    apply_fun Subtype.val at wc
+--    simp only [Icc.zero_val, Icc.succOfIndex_val, zero_add, Icc.end'_val] at wc
+--    rw [Icc.zero_val] at w0c
+--    rw [eq_comm, List.length_eq_one_iff] at wc
+--    rcases wc with ⟨a, wa⟩
+--    have wa' := congrArg (·[0]?) wa
+--    simp only [w0c, List.length_cons, List.length_nil, zero_add, zero_lt_one,
+--      getElem?_pos, List.getElem_cons_zero, Option.some.injEq] at wa'
+--    exact wa' ▸ wa
+--  · simp [wc] at w0c
+--  · simp [failure]
+--
+--theorem match'_concat (q r : Regex α) (w : List α)
+--    : match' [/¥ᵣ(q)¥ᵣ(r)/] w = (matchPartial q w 0 0).findSome?
+--        (fun (s, cap) ↦ matchFinish r w s cap) := by
+--  simp only [match', matchFinish, matchPartial, List.pure_def, List.bind_eq_flatMap,
+--    List.find?_flatMap, List.find?_singleton, decide_eq_true_eq, Option.map_eq_map,
+--    List.map_findSome?]
+--  congr
+--  rw [Function.comp_def]
+--  ext x cs
+--  rw [Option.map_eq_some_iff, Option.map_eq_some_iff]
+--  simp only [Prod.exists, exists_eq_right]
+--  simp only [List.findSome?_eq_some_iff, Option.ite_none_right_eq_some, Option.some.injEq,
+--    Prod.mk.injEq, ite_eq_right_iff, reduceCtorEq, imp_false, Prod.forall,
+--    exists_and_right, Prod.exists, ↓existsAndEq, and_true]
+--  rw [exists_comm]
+--  apply exists_congr; intro s
+--  simp only [List.find?_eq_some_iff_append, decide_eq_true_eq, Bool.not_eq_eq_eq_not,
+--    Bool.not_true, decide_eq_false_iff_not, Prod.forall, exists_and_right,
+--    ← Icc.val_inj]
+--  rw [← exists_and_left]
+--  apply exists_congr; intro csl
+--  rw [and_left_comm]
+--  rfl
+--
+--theorem match'_or (q r : Regex α) (w : List α)
+--    : match' (or q r) w = (match' q w <|> match' r w) := by
+--  simp only [match', matchFinish, matchPartial, List.find?_append, Option.map_eq_map,
+--    Option.orElse_eq_orElse, Option.orElse_eq_or]
+--  rw [Option.map_or]
+--
+--/-- Matching specialized to strings. -/
+--def matchStr (r : Regex Char) (w : String) := match' r w.toList
+--
+--def isMatch (r : Regex α) (w : List α) := ∃ cs, match' r w = some cs
+--
+--theorem isMatch_bot (w : List α) : ¬isMatch [/⊥/] w := by
+--  simp [isMatch, match'_bot]
+--
+--theorem isMatch_empty (w : List α) : isMatch [//] w ↔ w = [] := by
+--  simp [isMatch, match'_empty]
+--
+--theorem isMatch_unit (c : α) (w : List α) : isMatch [/c/] w ↔ w = [c] := by
+--  simp [isMatch, match'_unit]
+--
+--theorem isMatch_or (q r : Regex α) (w : List α)
+--    : isMatch (or q r) w ↔ isMatch q w ∨ isMatch r w := by
+--  simp only [isMatch, match'_or, Option.orElse_eq_orElse, Option.orElse_eq_or,
+--    Option.or_eq_some_iff]
+--  constructor <;> intro excs
+--  · rcases excs with ⟨cs, qcs | ⟨q0, rcs⟩⟩
+--    · exact Or.inl ⟨cs, qcs⟩
+--    · exact Or.inr ⟨cs, rcs⟩
+--  · by_cases qcs : ∃ cs, q.match' w = some cs
+--    · rcases qcs with ⟨cs, qcs⟩
+--      exact ⟨cs, Or.inl qcs⟩
+--    · simp only [qcs, false_or] at excs
+--      push_neg at qcs
+--      rw [← Option.eq_none_iff_forall_ne_some] at qcs
+--      rcases excs with ⟨cs, rcs⟩
+--      exact ⟨cs, Or.inr ⟨qcs, rcs⟩⟩
+--
+--def language (r : Regex α) : Language α := {w | isMatch r w}
+--
+--theorem language_bot (α : Type*) [DecidableEq α] : ([/⊥/] : Regex α).language = 0 := by
+--  simp [language, isMatch_bot]
+--  rfl
+--
+--theorem language_empty (α : Type*) [DecidableEq α] : ([//] : Regex α).language = {[]} := by
+--  simp [language, isMatch_empty]
+--
+--theorem language_unit (c : α) : [/c/].language = {[c]} := by
+--  simp [language, isMatch_unit]
+--
+--theorem language_or (q r : Regex α) : (or q r).language = q.language + r.language := by
+--  simp [language, isMatch_or, Language.add_def, Set.union_def]
+--
+--#eval matchStr [/(1 ← ('0' | '1')*) \⊥1/] "011011"
 
 end Regex
